``` LaTeX
$$ \begin{align*}
&  \operatorname{\int \frac{\operatorname{dx}}{a^2 + x^2}\ =\ \frac{1}{a} \tan^{-1} \bigg(\frac{x}{a}\bigg)} \\[1.3em]
&  \operatorname{\int \frac{\operatorname{dx}}{1 + x^2}\ =\ \tan^{-1} (x)} \\[1.3em]
&  \operatorname{\int \frac{\operatorname{dx}}{\sqrt{a^2 - x^2}}\ =\ \sin^{-1} \bigg(\frac{x}{a}\bigg)}  \\[1.3em]
&  \operatorname{\int \frac{\operatorname{dx}}{\sqrt{1 - x^2}}\ =\ \sin^{-1} (x)}  \\[1.3em]
&  \operatorname{\int \frac{\operatorname{dx}}{x\sqrt{x^2 - a^2}}\ =\ \frac{1}{a}  \sec^{-1} \bigg(\frac{x}{a}\bigg)}  \\[1.3em]
&  \operatorname{\int \frac{\operatorname{dx}}{x\sqrt{x^2 - 1}}\ =\  \sec^{-1}\ (x)}  \\[4em]




&  \operatorname{\int \frac{dx}{a^2- x^2}\ =\ \frac{1}{2a}
 \ln \bigg|\frac{a+x}{a-x} \bigg| }  \\[1.5em]
&  \operatorname{\int \frac{dx}{x^2-a^2}\ =\ \frac{1}{2a}
 \ln \bigg|\frac{x-a}{x+a} \bigg|} \\[1.5em]
&  \operatorname{\int \frac{dx}{1- x^2}\ =\ \frac{1}{2}  
 \ln \bigg|\frac{1+x}{1-x} \bigg| }  \\[1.5em]
&  \operatorname{\int \frac{dx}{x^2-1}\ =\ \frac{1}{2}
 \ln \bigg|\frac{x-1}{x+1} \bigg|}  \\[1.5em]
\end{align*}  $$


$$  \begin{align*}
&  \operatorname{\int \frac{dx}{\sqrt{x^2+a^2}} \ =\ \ln (x\ +\ \sqrt{x^2+a^2\ }) }  \\[1.5em]
&  \operatorname{\int \frac{dx}{\sqrt{x^2-a^2}} \ =\ \ln (x\ +\ \sqrt{x^2-a^2\ }) }\\[1.5em]  

&  \operatorname{\int \frac{dx}{\sqrt{x^2+1}} \ =\ \ln (x\ +\ \sqrt{x^2+1}) } \\[1.5em]
&  \operatorname{\int \frac{dx}{\sqrt{x^2-1}} \ =\ \ln (x\ +\ \sqrt{x^2-1}) } 
\end{align*} $$
$$  \\[3em]  $$

$$  \begin{align*}
&  \operatorname{\int \sqrt{x^2+a^2} \  \operatorname{dx} =\ \frac{x\sqrt{x^2+a^2}}{2}\ +\ \frac{a^2}{2}} \
\operatorname{\ln(x\ +\ \sqrt{x^2+a^2}) }  \\[1.3em]
&  \operatorname{\int \sqrt{x^2-a^2}} \ \operatorname{dx} = \operatorname{\frac{x\sqrt{x^2-a^2}}{2}} - \operatorname{\frac{a^2}{2} \
\ln(x\ +\ \sqrt{x^2-a^2})}  \\[1.5em]

&  \operatorname{\int \sqrt{a^2-x^2}\ dx\ =\ \frac{x\sqrt{a^2-x^2}}{2}\ +\ \frac{a^2}{2} \sin^{-1} \frac{x}{a} }  \\[3em]
\end{align*}  $$
```
